Move crash invariants to separate file.

src/program_logic/crash_weakestpre.v
@@ -98,10 +98,7 @@ Definition wpc_pre `{!irisG Λ Σ} (s : stuckness) (k: nat)
           [∗ list] i ↦ ef ∈ efs, wpc ⊤ ∅ ef fork_post True))
            ∧ |={∅}=> Φc ∗ |={∅, E2}=> state_interp σ1 (κ ++ κs) n))
    end ∧
-   match to_val e1 with
-   | Some v => |={E1, ∅}=> |={∅, ∅}▷=>^(S k) |={∅, ∅}=> Φc ∗ |={∅, E2}=> emp
-   | None => |={E1, ∅}=> |={∅, ∅}▷=>^(S k) |={∅, ∅}=> Φc ∗ |={∅, E2}=> emp
-   end)%I.
+   |={E1, ∅}=> |={∅, ∅}▷=>^(S k) |={∅, ∅}=> Φc ∗ |={∅, E2}=> emp)%I.
 
 
 Local Instance wpc_pre_contractive `{!irisG Λ Σ} s k : Contractive (wpc_pre s k).
@@ -177,8 +174,7 @@ Proof.
   (* FIXME: reflexivity, as being called many times by f_equiv and f_contractive
   is very slow here *)
   do 3 (apply step_fupdN_ne || f_contractive || f_equiv); auto; last first.
-  { apply step_fupdN_ne. repeat (f_contractive || f_equiv). auto. }
-  { apply step_fupdN_ne. repeat (f_contractive || f_equiv). auto. }
+  { repeat (f_contractive || f_equiv). auto. }
   do 12 (apply step_fupdN_ne || f_contractive || f_equiv); last first.
   { repeat (f_contractive || f_equiv). auto. }
   do 9 (apply step_fupdN_ne || f_contractive || f_equiv); last first.
@@ -202,13 +198,13 @@ Lemma wp_wpc s E1 E2 e Φ k:
   WP e @ s ; E1 {{ Φ }} ⊢ WPC e @ s ; k ; E1 ; E2 {{ Φ }} {{ True }}.
 Proof.
   iIntros (Hsub) "H". iLöb as "IH" forall (E1 E2 e Φ Hsub).
-  rewrite wp_unfold wpc_unfold /wp_pre /wpc_pre. destruct (to_val e) as [v|]=>//.
-  - iSplit; first auto. iMod "H".
-    iMod (fupd_intro_mask' _ ∅) as "Hclo"; first by set_solver+.
+  rewrite wp_unfold wpc_unfold /wp_pre /wpc_pre.
+  iSplit; last first.
+  - iMod (fupd_intro_mask' _ ∅) as "Hclo"; first by set_solver+.
     iApply step_fupdN_inner_later; auto. do 2 iNext.
     iSplitL ""; first auto.
     iMod "Hclo". iApply fupd_mask_weaken; eauto.
-  - iSplit.
+  - destruct (to_val e) as [v|]=>//.
     * iIntros (σ1 κ κs n) "Hσ".
       iMod (fupd_intro_mask' _ ∅) as "Hclo"; first by set_solver+.
       iModIntro.
@@ -228,10 +224,6 @@ Proof.
          iIntros "!#" (? ef _) "H". by iApply "IH".
       ** iModIntro. iSplitR; first done.
          iMod "Hclo". iApply fupd_mask_weaken; auto.
-    * iMod (fupd_intro_mask' _ ∅) as "Hclo"; first by set_solver+.
-      iModIntro. iApply step_fupdN_later; first reflexivity.
-      do 2 iNext. iModIntro. iSplitR; first done. iMod "Hclo" as "_".
-      iApply fupd_mask_weaken; auto.
 Qed.
 
 Lemma wpc_strong_mono s1 s2 k1 k2 E1 E2 E1' E2' e Φ Ψ Φc Ψc :
@@ -373,18 +365,6 @@ Lemma wpc_fupd s k E1 E2 e Φ Φc:
   ( WPC e @ s; k; E1 ; E2 {{ v, |={E1}=> Φ v }} {{ Φc }}) ⊢ WPC e @ s; k; E1 ; E2 {{ Φ }} {{ Φc }}.
 Proof. iIntros "H". iApply (wpc_strong_mono with "H"); auto. Qed.
 
-Axiom Tok: iProp Σ.
-Axiom Tok_Tok : Tok ∗ Tok -∗ False.
-Instance timeless_Tok: Timeless (Tok).
-Admitted.
-
-Context `{!stagedG Σ}.
-
-Definition detached_staged k E1 E2 P : iProp Σ :=
-  (|={E1, ∅}=> |={∅, ∅}▷=>^k |={∅, E2}=> P)%I.
-
-Definition detached_ci k E1 E2 N (P: iProp Σ) : iProp Σ :=
-  P ∨ (∃ γ, Tok ∗ staged_inv N γ (detached_staged k E1 E2 P))%I.
 
 Lemma wpc_crash s E1 E2 e k Φ Φc:
   WPC e @ s; k; E1 ; E2 {{ Φ }} {{ Φc }} -∗
@@ -394,364 +374,6 @@ Proof.
   rewrite wpc_unfold /wpc_pre.
   iDestruct "H" as "(_&H)".
   destruct (to_val e) as [v|]; auto.
-Qed.
-
-Lemma wpc_staged_invariant_aux s k E1 E2 E1' E2' e Φ Φc P Q1 R1 Q2 R2 N1 N2 γ :
-  ↑N1 ⊆ E1 →
-  ↑N2 ⊆ E1 →
-  (E2' ⊆ E1') →
-  (E1 ⊆ E1') →
-  (E2' ⊆ E2) →
-  N1 ## N2 →
-  inv N1 (detached_ci (2 * S (S (S k))) E1' E2' N2 P) ∗
-  □ (Q1 -∗ R1) ∗
-  □ (Q2 -∗ R2) ∗
-  staged_inv N2 γ (detached_staged (2 * (S (S (S k)))) E1' E2' P) ∗
-  staged_value N2 γ (|={E1 ∖ ↑N1 ∖ ↑N2, ∅}=> |={∅, ∅}▷=>^(S k)
-                     |={∅, E1 ∖ ↑N1 ∖ ↑N2}=>
-                     Q1 ∗ WPC e @ k; E1 ∖ ↑N1 ∖ ↑N2;E2 {{ v, (Φ v ∧ |={E1,E2}=> Φc) ∗ P }}{{Φc ∗ P}} ∗ Q2) ⊢
-  |={E1, ∅}=> |={∅, ∅}▷=>^(S (S (S k))) |={∅, E1}=> R1 ∗ WPC e @ s; S (S k); E1; E2 {{ v, Φ v }} {{Φc}} ∗ R2.
-Proof.
-  iIntros (????? Hdisj) "(#Hinv&#HQR1&#HQR2&#Hsi&Hwp)".
-  iLöb as "IH" forall (Q1 Q2 R1 R2 e) "HQR1 HQR2".
-  destruct (to_val e) as [v|] eqn:Hval.
-  {
-    rewrite Nat_iter_S.
-    iMod (staged_inv_open with "[$]") as "(H&Hclo')".
-    { set_solver. }
-    iMod (fupd_intro_mask' _ ∅) as "Hclo"; first by set_solver+.
-    iModIntro. rewrite Nat_iter_S. iModIntro. iNext. iModIntro.
-    rewrite Nat_iter_S.
-    iModIntro. iNext.
-    iMod "Hclo" as "_".
-    iMod (fupd_intro_mask' _ (E1 ∖ ↑N1 ∖ ↑N2)) as "Hclo"; first by set_solver+.
-    iMod "H". iModIntro.
-    rewrite Nat_iter_S. iMod "H".  iModIntro. iNext. iMod "H". iModIntro.
-    iApply (step_fupdN_wand with "H").
-    iIntros "H".
-    iMod "H".
-    rewrite wpc_unfold /wpc_pre.
-    rewrite wpc_unfold /wpc_pre.
-    rewrite Hval. iDestruct "H" as "(HQ1&(H&_)&HQ2)".
-    iMod "H" as "(HΦ&HP)".
-    iMod "Hclo".
-    iMod ("Hclo'" with "[HP]").
-    { iSplitL. iApply "HP". iAlways.
-      iIntros. rewrite /detached_staged.
-      iApply step_fupdN_inner_later; first auto.
-      iNext. eauto.
-    }
-    iModIntro.
-    iSplitL "HQ1".
-    { by iApply "HQR1". }
-    iSplitR "HQ2"; last first.
-    { by iApply "HQR2". }
-    iSplit.
-    - by iDestruct "HΦ" as "($&_)".
-    - iDestruct "HΦ" as "(_&HΦ)".
-      iMod "HΦ". iMod (fupd_intro_mask' _ ∅) as "?"; first by set_solver.
-      iModIntro.
-      iApply step_fupdN_later; first by set_solver.
-      repeat iNext. by iFrame.
-  }
-  rewrite (Nat_iter_S ((S (S k)))).
-  iMod (staged_inv_open with "[$]") as "(H&Hclo')".
-  { set_solver. }
-  iMod (fupd_intro_mask' _ ∅) as "Hclo"; first by set_solver+.
-  rewrite (Nat_iter_S (S k)).
-  iModIntro. iModIntro. iNext. iModIntro.
-  iModIntro. iNext.
-  iMod "Hclo" as "_".
-  iMod (fupd_intro_mask' _ (E1 ∖ ↑N1 ∖ ↑N2)) as "Hclo"; first by set_solver+.
-  iMod "H". iModIntro.
-  iApply (step_fupdN_wand with "H").
-  iIntros "H".
-  iMod "H".
-  iMod "Hclo" as "_".
-  iDestruct "H" as "(HQ1&H&HQ2)".
-  iSpecialize ("Hclo'" $! _ with "[H]").
-  { iSplitL "H". iApply "H".
-    iAlways.
-    iIntros "H".
-    rewrite wpc_unfold /wpc_pre.
-    rewrite Hval. iDestruct "H" as "(_&HP)".
-    rewrite /detached_staged.
-    iMod (fupd_intro_mask') as "Hclo"; [| iMod "HP"].
-    { set_solver. }
-    iModIntro.
-    iApply (step_fupdN_le (S k)).
-    { reflexivity. }
-    { lia. }
-    iApply (step_fupdN_wand with "HP").
-    iIntros "HP". iMod "HP". iDestruct "HP" as "((_&HP)&Hclo')".
-    iMod "Hclo'".
-    iApply fupd_mask_weaken; auto.
-  }
-  iMod "Hclo'".
-  iModIntro.
-  iSplitL "HQ1".
-  { iApply "HQR1". eauto. }
-  iSplitR "HQ2"; last first.
-  { iApply "HQR2". eauto. }
-  rewrite wpc_unfold /wpc_pre. rewrite Hval.
-  iSplit.
-  - iIntros.
-    iMod (staged_inv_open with "[$]") as "(H&Hclo')".
-    { set_solver. }
-    iMod (fupd_intro_mask' _ ∅) as "Hclo''".
-    { set_solver. }
-    iModIntro. rewrite Nat_iter_S. rewrite Nat_iter_S.
-    iModIntro. iNext. iModIntro. iModIntro. iNext.
-    iMod "Hclo''" as "_".
-    rewrite wpc_unfold /wpc_pre.
-    rewrite Hval. iDestruct "H" as "(H&_)".
-    iMod (fupd_intro_mask' _ (E1 ∖ ↑N1 ∖ ↑N2)) as "Hclo''".
-    { set_solver. }
-    iMod ("H" with "[$]") as "H".
-    iModIntro.
-    iApply (step_fupdN_wand with "H").
-    iIntros "H".
-    iSplit; last first.
-    { iDestruct "H" as "(_&H)".
-      iMod "H" as "(($&?)&$)". eauto.
-    }
-    iDestruct "H" as "(H&_)".
-    iMod "H". iModIntro.
-    iDestruct "H" as "(%&H)".
-    iSplitL "".
-    { destruct s; eauto. }
-    iIntros.
-    iMod ("H" with "[//]") as "H".
-    iModIntro. iNext. iMod "H" as "H".
-
-    iMod "Hclo''" as "_".
-    iSpecialize ("Hclo'" $! _ with "[H]").
-    { iSplitL "H". iApply "H".
-      iAlways. iIntros "H".
-      rewrite /detached_staged.
-      replace (2 * S (S (S k))) with (S (S (S k)) + S (S (S k))) by lia.
-      iApply step_fupdN_inner_plus.
-      iMod (fupd_intro_mask' _ (E1 ∖ ↑N1 ∖ ↑N2)) as "Hclo''".
-      { set_solver. }
-      iMod "H".
-      iModIntro.
-      iApply (step_fupdN_le (S k)); first reflexivity.
-      { lia. }
-      iApply (step_fupdN_wand with "H"). iIntros "H".
-      iMod "H". iMod "Hclo''" as "_".
-      iDestruct "H" as "(_&H&_)".
-      iPoseProof (wpc_crash with "H") as "H".
-      iModIntro.
-      iMod (fupd_intro_mask') as "Hclo"; [| iMod "H"].
-      { set_solver. }
-      iModIntro.
-      iApply (step_fupdN_le (S k)).
-      { reflexivity. }
-      { lia. }
-      iApply (step_fupdN_wand with "H").
-      iIntros "HP". iMod "HP". iDestruct "HP" as "((_&HP)&Hclo')".
-      iMod "Hclo'".
-      iApply fupd_mask_weaken; auto.
-    }
-    iMod "Hclo'". iModIntro.
-    iApply ("IH" with "Hclo' [] []").
-    { iAlways. iIntros "H". eauto. }
-    { iAlways. iIntros "H". iApply (big_sepL_mono with "H").
-      iIntros. iApply (wpc_strong_mono with "[$]"); eauto.
-    }
-  - iIntros.
-    iMod (staged_inv_open with "[$]") as "(H&Hclo')".
-    { set_solver. }
-    iMod (fupd_intro_mask' _ ∅) as "Hclo''".
-    { set_solver. }
-    iModIntro. rewrite Nat_iter_S. rewrite Nat_iter_S.
-    iModIntro. iNext. iModIntro. iModIntro. iNext.
-    iMod "Hclo''" as "_".
-    rewrite wpc_unfold /wpc_pre.
-    rewrite Hval. iDestruct "H" as "(_&H)".
-    iMod (fupd_intro_mask' _ (E1 ∖ ↑N1 ∖ ↑N2)) as "Hclo''".
-    { set_solver. }
-    iMod ("H") as "H".
-    iModIntro.
-    iApply (step_fupdN_wand with "H").
-    iIntros "H".
-    iMod "H" as "(($&HP)&$)".
-    eauto.
-Qed.
-
-Lemma detached_ci_tok k E1 E2 N P:
-  ▷ detached_ci k E1 E2 N P -∗
-  Tok -∗
-  ▷ (P ∗ Tok).
-Proof.
-  iIntros "HCI HTok".
-  iNext.
-  rewrite /detached_ci.
-  iDestruct "HCI" as "[$|H]".
-  - iFrame.
-  - iDestruct "H" as (?) "(H&?)".
-    iDestruct (Tok_Tok with "[$]") as "[]".
-Qed.
-
-Lemma wpc_staged_invariant s k E1 E2 E1' E2' e Φ Φc P N1 N2 :
-  ↑N1 ⊆ E1 →
-  ↑N2 ⊆ E1 →
-  (E2' ⊆ E1') →
-  (E1 ⊆ E1') →
-  (E2' ⊆ E2) →
-  N1 ## N2 →
-  inv N1 (detached_ci (2 * S (S (S k))) E1' E2' N2 P) ∗
-  Tok ∗
-  (▷ (P) -∗ WPC e @ NotStuck; k; (E1 ∖ ↑N1 ∖ ↑N2); E2
-                {{ λ v, (Φ v ∧ |={E1,E2}=> Φc) ∗ P}} {{ Φc ∗ P }}) ⊢
-  WPC e @ s; (S (S k)); E1; E2 {{ Φ }} {{ Φc }}.
-Proof.
-  iIntros (????? Hdisj) "(#Hinv&Htok&Hwp)".
-  rewrite !wpc_unfold /wpc_pre.
-  iSplit; last first.
-  {
-    destruct (to_val e).
-    - iInv "Hinv" as "H" "Hclo".
-      iDestruct (detached_ci_tok with "[$] [$]") as "(H&Htok)".
-      iDestruct ("Hwp" with "[$]") as "(_&H)".
-      iIntros.
-      iMod (fupd_intro_mask' _ (E1 ∖ ↑N1 ∖ ↑N2)) as "Hclo'".
-      { set_solver. }
-      iMod "H". iModIntro.
-      iApply (step_fupdN_le (S k)); first by set_solver+.
-      { lia. }
-      iApply (step_fupdN_wand with "H").
-      iIntros "H". iMod "H" as "(($&?)&$)".
-      eauto.
-    - iInv "Hinv" as "H" "Hclo".
-      iDestruct (detached_ci_tok with "[$] [$]") as "(H&Htok)".
-      iDestruct ("Hwp" with "[$]") as "(_&H)".
-      iIntros.
-      iMod (fupd_intro_mask' _ (E1 ∖ ↑N1 ∖ ↑N2)) as "Hclo'".
-      { set_solver. }
-      iMod "H". iModIntro.
-      iApply (step_fupdN_le (S k)); first by set_solver+.
-      { lia. }
-      iApply (step_fupdN_wand with "H").
-      iIntros "H". iMod "H" as "(($&?)&$)".
-      eauto.
-  }
-  destruct (to_val e).
-  - iInv "Hinv" as "H" "Hclo".
-    iDestruct (detached_ci_tok with "[$] [$]") as "(H&Htok)".
-    iMod (fupd_intro_mask' _ (E1 ∖ ↑N1 ∖ ↑N2)) as "Hclo'".
-    { set_solver+. }
-    iDestruct ("Hwp" with "[$]") as "(H&_)".
-    iMod "H" as "(($&_)&HP)".
-    iMod "Hclo'".
-    iMod ("Hclo" with "[-]"); last eauto.
-    iLeft. iFrame.
-  - iIntros (????) "Hstate".
-    iInv "Hinv" as "H" "Hclo".
-    iDestruct (detached_ci_tok with "[$] [$]") as "(H&Htok)".
-    iDestruct ("Hwp" with "[$]") as "(Hwp&_)".
-    replace (↑ N2 : coPset) with (∅ ∪ ↑N2 : coPset) at 1 by set_solver.
-    replace (E1 ∖ ↑N1) with (((E1 ∖ ↑N1) ∖ ↑N2) ∪ ↑N2) at 2; last first.
-    { assert ((↑N1: coPset) ## (↑N2: coPset)). set_solver.
-      clear Hdisj.
-      assert (↑N2 ⊆ E1 ∖ ↑N1) by set_solver.
-      rewrite difference_union_L. set_solver.
-    }
-    iSpecialize ("Hwp" with "[$]").
-    iMod (fupd_mask_frame_r with "Hwp") as "Hwp".
-    { set_solver. }
-    rewrite left_id_L.
-    iMod (fupd_intro_mask' (↑N2) ∅) as "Hclo'".
-    { set_solver. }
-    iModIntro. do 2 iEval (rewrite Nat_iter_S_r).
-    iApply (step_fupdN_wand with "Hwp").
-    iIntros "Hwp".
-    iMod (staged_inv_alloc N2 _
-             (|={E1', ∅}=> |={∅, ∅}▷=>^(2 * S (S (S k))) |={∅, E2'}=>P)%I _ with "[Hwp]")
-      as (γ) "(#Hsi&Hval)".
-    { iSplitL "Hwp". iApply "Hwp".
-       iAlways. iIntros "(_&Hwp)".
-       iMod (fupd_intro_mask' _ ∅) as "Hclo"; first by set_solver+.
-       iMod "Hwp".
-       iModIntro.
-       iApply step_fupdN_later; eauto.
-       iNext. iDestruct "Hwp" as "((?&HP)&Hclo')".
-       iMod "Hclo" as "_". iApply fupd_mask_weaken; eauto.
-    }
-    iMod "Hclo'" as "_".
-    iMod (staged_inv_open with "[$]") as "(H&Hclo')".
-    { set_solver. }
-    rewrite difference_diag_L.
-    iModIntro. iNext. iModIntro. iModIntro. iNext.
-    iModIntro.
-    iSplit.
-    *
-    iDestruct "H" as "(H&_)".
-    iMod "H". iModIntro.
-    iDestruct "H" as "(%&H)".
-    iSplitL "".
-    { destruct s; eauto. }
-    iIntros.
-    iMod ("H" with "[//]") as "H".
-    iModIntro. iNext. iMod "H" as "H".
-    iSpecialize ("Hclo'" $! _ with "[H]").
-    { iSplitL "H". iApply "H".
-      iAlways.
-      iIntros "H".
-
-      replace (2 * S (S (S k))) with (S (S (S k)) + S (S (S k))) by lia.
-      iApply step_fupdN_inner_plus.
-      iMod (fupd_intro_mask' _ (E1 ∖ ↑N1 ∖ ↑N2)) as "Hclo''".
-      { set_solver. }
-      iMod "H".
-      iModIntro.
-      iApply (step_fupdN_le (S k)); first reflexivity.
-      { lia. }
-      iApply (step_fupdN_wand with "H"). iIntros "H".
-      iMod "H". iMod "Hclo''" as "_".
-      iDestruct "H" as "(_&H&_)".
-      iPoseProof (wpc_crash with "H") as "H".
-      iModIntro.
-      iMod (fupd_intro_mask') as "Hclo"; [| iMod "H"].
-      { set_solver. }
-      iModIntro.
-      iApply (step_fupdN_le (S k)).
-      { reflexivity. }
-      { lia. }
-      iApply (step_fupdN_wand with "H").
-      iIntros "HP". iMod "HP". iDestruct "HP" as "((_&HP)&Hclo')".
-      iMod "Hclo'".
-      iApply fupd_mask_weaken; auto.
-    }
-    iAssert (|={E1 ∖ ↑N1 ∖ ↑N2,E1 ∖ ↑N1}=> staged_value N2 γ _)%I with "[Hclo']" as "H".
-    {
-    iApply fupd_mask_frame.
-    2: { iMod "Hclo'". iModIntro.
-         rewrite difference_empty_L.
-         iApply (fupd_mask_same).
-         rewrite (comm_L (∪)).
-      assert (↑N2 ⊆ E1 ∖ ↑N1) by set_solver.
-      rewrite difference_union_L. set_solver.
-      iModIntro. eauto.
-    }
-    { set_solver. }
-    }
-    iMod "H".
-    iMod ("Hclo" with "[Htok]") as "_".
-    { iNext. iRight. iExists _. iFrame. iFrame "Hsi". }
-    iModIntro.
-    iApply (wpc_staged_invariant_aux s k E1 E2 E1' E2'
-                  _ Φ Φc P
-                  (state_interp σ2 a1 (strings.length efs + a2)) _
-                  ([∗ list] ef ∈ efs, WPC ef @ k; ⊤;∅ {{ v, fork_post v }}{{True}})%I  _ N1 N2 with "[H]"); try assumption.
-    { iIntros. iFrame "Hinv". iFrame "H".
-      iFrame "Hsi". iSplit.
-      - eauto.
-      - iAlways. iIntros "H". iApply (big_sepL_mono with "H").
-        iIntros. iApply (wpc_strong_mono with "[$]"); eauto.
-    }
-    * iDestruct "H" as "(_&H)".
-      iMod "H" as "(($&_)&$)". eauto.
 Qed.
 
 (* XXX: the Atomic hypothesis could be weakened to
