src/program_logic/crash_inv.v
@@ -1,0 +1,383 @@
+From iris.proofmode Require Import base tactics classes.
+From iris.base_logic Require Export invariants.
+From iris.program_logic Require Export weakestpre.
+From Perennial.program_logic Require Import staged_invariant crash_weakestpre.
+Set Default Proof Using "Type".
+Import uPred.
+
+Section ci.
+Context `{!irisG Λ Σ}.
+Context `{!stagedG Σ}.
+
+Axiom Tok: iProp Σ.
+Axiom Tok_Tok : Tok ∗ Tok -∗ False.
+Instance timeless_Tok: Timeless (Tok).
+Admitted.
+
+
+Definition detached_staged k E1 E2 P : iProp Σ :=
+  (|={E1, ∅}=> |={∅, ∅}▷=>^k |={∅, E2}=> P)%I.
+
+Definition detached_ci k E1 E2 N (P: iProp Σ) : iProp Σ :=
+  P ∨ (∃ γ, Tok ∗ staged_inv N γ (detached_staged k E1 E2 P))%I.
+
+Lemma wpc_staged_invariant_aux s k E1 E2 E1' E2' e Φ Φc P Q1 R1 Q2 R2 N1 N2 γ :
+  ↑N1 ⊆ E1 →
+  ↑N2 ⊆ E1 →
+  (E2' ⊆ E1') →
+  (E1 ⊆ E1') →
+  (E2' ⊆ E2) →
+  N1 ## N2 →
+  inv N1 (detached_ci (2 * S (S (S k))) E1' E2' N2 P) ∗
+  □ (Q1 -∗ R1) ∗
+  □ (Q2 -∗ R2) ∗
+  staged_inv N2 γ (detached_staged (2 * (S (S (S k)))) E1' E2' P) ∗
+  staged_value N2 γ (|={E1 ∖ ↑N1 ∖ ↑N2, ∅}=> |={∅, ∅}▷=>^(S k)
+                     |={∅, E1 ∖ ↑N1 ∖ ↑N2}=>
+                     Q1 ∗ WPC e @ k; E1 ∖ ↑N1 ∖ ↑N2;E2 {{ v, (Φ v ∧ |={E1,E2}=> Φc) ∗ P }}{{Φc ∗ P}} ∗ Q2) ⊢
+  |={E1, ∅}=> |={∅, ∅}▷=>^(S (S (S k))) |={∅, E1}=> R1 ∗ WPC e @ s; S (S k); E1; E2 {{ v, Φ v }} {{Φc}} ∗ R2.
+Proof.
+  iIntros (????? Hdisj) "(#Hinv&#HQR1&#HQR2&#Hsi&Hwp)".
+  iLöb as "IH" forall (Q1 Q2 R1 R2 e) "HQR1 HQR2".
+  destruct (to_val e) as [v|] eqn:Hval.
+  {
+    rewrite Nat_iter_S.
+    iMod (staged_inv_open with "[$]") as "(H&Hclo')".
+    { set_solver. }
+    iMod (fupd_intro_mask' _ ∅) as "Hclo"; first by set_solver+.
+    iModIntro. rewrite Nat_iter_S. iModIntro. iNext. iModIntro.
+    rewrite Nat_iter_S.
+    iModIntro. iNext.
+    iMod "Hclo" as "_".
+    iMod (fupd_intro_mask' _ (E1 ∖ ↑N1 ∖ ↑N2)) as "Hclo"; first by set_solver+.
+    iMod "H". iModIntro.
+    rewrite Nat_iter_S. iMod "H".  iModIntro. iNext. iMod "H". iModIntro.
+    iApply (step_fupdN_wand with "H").
+    iIntros "H".
+    iMod "H".
+    rewrite wpc_unfold /wpc_pre.
+    rewrite wpc_unfold /wpc_pre.
+    rewrite Hval. iDestruct "H" as "(HQ1&(H&_)&HQ2)".
+    iMod "H" as "(HΦ&HP)".
+    iMod "Hclo".
+    iMod ("Hclo'" with "[HP]").
+    { iSplitL. iApply "HP". iAlways.
+      iIntros. rewrite /detached_staged.
+      iApply step_fupdN_inner_later; first auto.
+      iNext. eauto.
+    }
+    iModIntro.
+    iSplitL "HQ1".
+    { by iApply "HQR1". }
+    iSplitR "HQ2"; last first.
+    { by iApply "HQR2". }
+    iSplit.
+    - by iDestruct "HΦ" as "($&_)".
+    - iDestruct "HΦ" as "(_&HΦ)".
+      iMod "HΦ". iMod (fupd_intro_mask' _ ∅) as "?"; first by set_solver.
+      iModIntro.
+      iApply step_fupdN_later; first by set_solver.
+      repeat iNext. by iFrame.
+  }
+  rewrite (Nat_iter_S ((S (S k)))).
+  iMod (staged_inv_open with "[$]") as "(H&Hclo')".
+  { set_solver. }
+  iMod (fupd_intro_mask' _ ∅) as "Hclo"; first by set_solver+.
+  rewrite (Nat_iter_S (S k)).
+  iModIntro. iModIntro. iNext. iModIntro.
+  iModIntro. iNext.
+  iMod "Hclo" as "_".
+  iMod (fupd_intro_mask' _ (E1 ∖ ↑N1 ∖ ↑N2)) as "Hclo"; first by set_solver+.
+  iMod "H". iModIntro.
+  iApply (step_fupdN_wand with "H").
+  iIntros "H".
+  iMod "H".
+  iMod "Hclo" as "_".
+  iDestruct "H" as "(HQ1&H&HQ2)".
+  iSpecialize ("Hclo'" $! _ with "[H]").
+  { iSplitL "H". iApply "H".
+    iAlways.
+    iIntros "H".
+    rewrite wpc_unfold /wpc_pre.
+    rewrite Hval. iDestruct "H" as "(_&HP)".
+    rewrite /detached_staged.
+    iMod (fupd_intro_mask') as "Hclo"; [| iMod "HP"].
+    { set_solver. }
+    iModIntro.
+    iApply (step_fupdN_le (S k)).
+    { reflexivity. }
+    { lia. }
+    iApply (step_fupdN_wand with "HP").
+    iIntros "HP". iMod "HP". iDestruct "HP" as "((_&HP)&Hclo')".
+    iMod "Hclo'".
+    iApply fupd_mask_weaken; auto.
+  }
+  iMod "Hclo'".
+  iModIntro.
+  iSplitL "HQ1".
+  { iApply "HQR1". eauto. }
+  iSplitR "HQ2"; last first.
+  { iApply "HQR2". eauto. }
+  iEval (rewrite wpc_unfold /wpc_pre). rewrite Hval.
+  iSplit.
+  - iIntros.
+    iMod (staged_inv_open with "[$]") as "(H&Hclo')".
+    { set_solver. }
+    iMod (fupd_intro_mask' _ ∅) as "Hclo''".
+    { set_solver. }
+    iModIntro. rewrite Nat_iter_S. rewrite Nat_iter_S.
+    iModIntro. iNext. iModIntro. iModIntro. iNext.
+    iMod "Hclo''" as "_".
+    rewrite wpc_unfold /wpc_pre.
+    rewrite Hval. iDestruct "H" as "(H&_)".
+    iMod (fupd_intro_mask' _ (E1 ∖ ↑N1 ∖ ↑N2)) as "Hclo''".
+    { set_solver. }
+    iMod ("H" with "[$]") as "H".
+    iModIntro.
+    iApply (step_fupdN_wand with "H").
+    iIntros "H".
+    iSplit; last first.
+    { iDestruct "H" as "(_&H)".
+      iMod "H" as "(($&?)&$)". eauto.
+    }
+    iDestruct "H" as "(H&_)".
+    iMod "H". iModIntro.
+    iDestruct "H" as "(%&H)".
+    iSplitL "".
+    { destruct s; eauto. }
+    iIntros.
+    iMod ("H" with "[//]") as "H".
+    iModIntro. iNext. iMod "H" as "H".
+
+    iMod "Hclo''" as "_".
+    iSpecialize ("Hclo'" $! _ with "[H]").
+    { iSplitL "H". iApply "H".
+      iAlways. iIntros "H".
+      rewrite /detached_staged.
+      replace (2 * S (S (S k))) with (S (S (S k)) + S (S (S k))) by lia.
+      iApply step_fupdN_inner_plus.
+      iMod (fupd_intro_mask' _ (E1 ∖ ↑N1 ∖ ↑N2)) as "Hclo''".
+      { set_solver. }
+      iMod "H".
+      iModIntro.
+      iApply (step_fupdN_le (S k)); first reflexivity.
+      { lia. }
+      iApply (step_fupdN_wand with "H"). iIntros "H".
+      iMod "H". iMod "Hclo''" as "_".
+      iDestruct "H" as "(_&H&_)".
+      iPoseProof (wpc_crash with "H") as "H".
+      iModIntro.
+      iMod (fupd_intro_mask') as "Hclo"; [| iMod "H"].
+      { set_solver. }
+      iModIntro.
+      iApply (step_fupdN_le (S k)).
+      { reflexivity. }
+      { lia. }
+      iApply (step_fupdN_wand with "H").
+      iIntros "HP". iMod "HP". iDestruct "HP" as "((_&HP)&Hclo')".
+      iMod "Hclo'".
+      iApply fupd_mask_weaken; auto.
+    }
+    iMod "Hclo'". iModIntro.
+    iApply ("IH" with "Hclo' [] []").
+    { iAlways. iIntros "H". eauto. }
+    { iAlways. iIntros "H". iApply (big_sepL_mono with "H").
+      iIntros. iApply (wpc_strong_mono with "[$]"); eauto.
+    }
+  - iIntros.
+    iMod (staged_inv_open with "[$]") as "(H&Hclo')".
+    { set_solver. }
+    iMod (fupd_intro_mask' _ ∅) as "Hclo''".
+    { set_solver. }
+    iModIntro. rewrite Nat_iter_S. rewrite Nat_iter_S.
+    iModIntro. iNext. iModIntro. iModIntro. iNext.
+    iMod "Hclo''" as "_".
+    rewrite wpc_unfold /wpc_pre.
+    rewrite Hval. iDestruct "H" as "(_&H)".
+    iMod (fupd_intro_mask' _ (E1 ∖ ↑N1 ∖ ↑N2)) as "Hclo''".
+    { set_solver. }
+    iMod ("H") as "H".
+    iModIntro.
+    iApply (step_fupdN_wand with "H").
+    iIntros "H".
+    iMod "H" as "(($&HP)&$)".
+    eauto.
+Qed.
+
+Lemma detached_ci_tok k E1 E2 N P:
+  ▷ detached_ci k E1 E2 N P -∗
+  Tok -∗
+  ▷ (P ∗ Tok).
+Proof.
+  iIntros "HCI HTok".
+  iNext.
+  rewrite /detached_ci.
+  iDestruct "HCI" as "[$|H]".
+  - iFrame.
+  - iDestruct "H" as (?) "(H&?)".
+    iDestruct (Tok_Tok with "[$]") as "[]".
+Qed.
+
+Lemma wpc_staged_invariant s k E1 E2 E1' E2' e Φ Φc P N1 N2 :
+  ↑N1 ⊆ E1 →
+  ↑N2 ⊆ E1 →
+  (E2' ⊆ E1') →
+  (E1 ⊆ E1') →
+  (E2' ⊆ E2) →
+  N1 ## N2 →
+  inv N1 (detached_ci (2 * S (S (S k))) E1' E2' N2 P) ∗
+  Tok ∗
+  (▷ (P) -∗ WPC e @ NotStuck; k; (E1 ∖ ↑N1 ∖ ↑N2); E2
+                {{ λ v, (Φ v ∧ |={E1,E2}=> Φc) ∗ P}} {{ Φc ∗ P }}) ⊢
+  WPC e @ s; (S (S k)); E1; E2 {{ Φ }} {{ Φc }}.
+Proof.
+  iIntros (????? Hdisj) "(#Hinv&Htok&Hwp)".
+  rewrite !wpc_unfold /wpc_pre.
+  iSplit; last first.
+  {
+    destruct (to_val e).
+    - iInv "Hinv" as "H" "Hclo".
+      iDestruct (detached_ci_tok with "[$] [$]") as "(H&Htok)".
+      iDestruct ("Hwp" with "[$]") as "(_&H)".
+      iIntros.
+      iMod (fupd_intro_mask' _ (E1 ∖ ↑N1 ∖ ↑N2)) as "Hclo'".
+      { set_solver. }
+      iMod "H". iModIntro.
+      iApply (step_fupdN_le (S k)); first by set_solver+.
+      { lia. }
+      iApply (step_fupdN_wand with "H").
+      iIntros "H". iMod "H" as "(($&?)&$)".
+      eauto.
+    - iInv "Hinv" as "H" "Hclo".
+      iDestruct (detached_ci_tok with "[$] [$]") as "(H&Htok)".
+      iDestruct ("Hwp" with "[$]") as "(_&H)".
+      iIntros.
+      iMod (fupd_intro_mask' _ (E1 ∖ ↑N1 ∖ ↑N2)) as "Hclo'".
+      { set_solver. }
+      iMod "H". iModIntro.
+      iApply (step_fupdN_le (S k)); first by set_solver+.
+      { lia. }
+      iApply (step_fupdN_wand with "H").
+      iIntros "H". iMod "H" as "(($&?)&$)".
+      eauto.
+  }
+  destruct (to_val e).
+  - iInv "Hinv" as "H" "Hclo".
+    iDestruct (detached_ci_tok with "[$] [$]") as "(H&Htok)".
+    iMod (fupd_intro_mask' _ (E1 ∖ ↑N1 ∖ ↑N2)) as "Hclo'".
+    { set_solver+. }
+    iDestruct ("Hwp" with "[$]") as "(H&_)".
+    iMod "H" as "(($&_)&HP)".
+    iMod "Hclo'".
+    iMod ("Hclo" with "[-]"); last eauto.
+    iLeft. iFrame.
+  - iIntros (????) "Hstate".
+    iInv "Hinv" as "H" "Hclo".
+    iDestruct (detached_ci_tok with "[$] [$]") as "(H&Htok)".
+    iDestruct ("Hwp" with "[$]") as "(Hwp&_)".
+    replace (↑ N2 : coPset) with (∅ ∪ ↑N2 : coPset) at 1 by set_solver.
+    replace (E1 ∖ ↑N1) with (((E1 ∖ ↑N1) ∖ ↑N2) ∪ ↑N2) at 2; last first.
+    { assert ((↑N1: coPset) ## (↑N2: coPset)). set_solver.
+      clear Hdisj.
+      assert (↑N2 ⊆ E1 ∖ ↑N1) by set_solver.
+      rewrite difference_union_L. set_solver.
+    }
+    iSpecialize ("Hwp" with "[$]").
+    iMod (fupd_mask_frame_r with "Hwp") as "Hwp".
+    { set_solver. }
+    rewrite left_id_L.
+    iMod (fupd_intro_mask' (↑N2) ∅) as "Hclo'".
+    { set_solver. }
+    iModIntro. do 2 iEval (rewrite Nat_iter_S_r).
+    iApply (step_fupdN_wand with "Hwp").
+    iIntros "Hwp".
+    iMod (staged_inv_alloc N2 _
+             (|={E1', ∅}=> |={∅, ∅}▷=>^(2 * S (S (S k))) |={∅, E2'}=>P)%I _ with "[Hwp]")
+      as (γ) "(#Hsi&Hval)".
+    { iSplitL "Hwp". iApply "Hwp".
+       iAlways. iIntros "(_&Hwp)".
+       iMod (fupd_intro_mask' _ ∅) as "Hclo"; first by set_solver+.
+       iMod "Hwp".
+       iModIntro.
+       iApply step_fupdN_later; eauto.
+       iNext. iDestruct "Hwp" as "((?&HP)&Hclo')".
+       iMod "Hclo" as "_". iApply fupd_mask_weaken; eauto.
+    }
+    iMod "Hclo'" as "_".
+    iMod (staged_inv_open with "[$]") as "(H&Hclo')".
+    { set_solver. }
+    rewrite difference_diag_L.
+    iModIntro. iNext. iModIntro. iModIntro. iNext.
+    iModIntro.
+    iSplit.
+    *
+    iDestruct "H" as "(H&_)".
+    iMod "H". iModIntro.
+    iDestruct "H" as "(%&H)".
+    iSplitL "".
+    { destruct s; eauto. }
+    iIntros.
+    iMod ("H" with "[//]") as "H".
+    iModIntro. iNext. iMod "H" as "H".
+    iSpecialize ("Hclo'" $! _ with "[H]").
+    { iSplitL "H". iApply "H".
+      iAlways.
+      iIntros "H".
+
+      replace (2 * S (S (S k))) with (S (S (S k)) + S (S (S k))) by lia.
+      iApply step_fupdN_inner_plus.
+      iMod (fupd_intro_mask' _ (E1 ∖ ↑N1 ∖ ↑N2)) as "Hclo''".
+      { set_solver. }
+      iMod "H".
+      iModIntro.
+      iApply (step_fupdN_le (S k)); first reflexivity.
+      { lia. }
+      iApply (step_fupdN_wand with "H"). iIntros "H".
+      iMod "H". iMod "Hclo''" as "_".
+      iDestruct "H" as "(_&H&_)".
+      iPoseProof (wpc_crash with "H") as "H".
+      iModIntro.
+      iMod (fupd_intro_mask') as "Hclo"; [| iMod "H"].
+      { set_solver. }
+      iModIntro.
+      iApply (step_fupdN_le (S k)).
+      { reflexivity. }
+      { lia. }
+      iApply (step_fupdN_wand with "H").
+      iIntros "HP". iMod "HP". iDestruct "HP" as "((_&HP)&Hclo')".
+      iMod "Hclo'".
+      iApply fupd_mask_weaken; auto.
+    }
+    iAssert (|={E1 ∖ ↑N1 ∖ ↑N2,E1 ∖ ↑N1}=> staged_value N2 γ _)%I with "[Hclo']" as "H".
+    {
+    iApply fupd_mask_frame.
+    2: { iMod "Hclo'". iModIntro.
+         rewrite difference_empty_L.
+         iApply (fupd_mask_same).
+         rewrite (comm_L (∪)).
+      assert (↑N2 ⊆ E1 ∖ ↑N1) by set_solver.
+      rewrite difference_union_L. set_solver.
+      iModIntro. eauto.
+    }
+    { set_solver. }
+    }
+    iMod "H".
+    iMod ("Hclo" with "[Htok]") as "_".
+    { iNext. iRight. iExists _. iFrame. iFrame "Hsi". }
+    iModIntro.
+    iApply (wpc_staged_invariant_aux s k E1 E2 E1' E2'
+                  _ Φ Φc P
+                  (state_interp σ2 a1 (strings.length efs + a2)) _
+                  ([∗ list] ef ∈ efs, WPC ef @ k; ⊤;∅ {{ v, fork_post v }}{{True}})%I  _ N1 N2 with "[H]"); try assumption.
+    { iIntros. iFrame "Hinv". iFrame "H".
+      iFrame "Hsi". iSplit.
+      - eauto.
+      - iAlways. iIntros "H". iApply (big_sepL_mono with "H").
+        iIntros. iApply (wpc_strong_mono with "[$]"); eauto.
+    }
+    * iDestruct "H" as "(_&H)".
+      iMod "H" as "(($&_)&$)". eauto.
+Qed.
+
+
+End ci.
